tuned

Examples/Example_Semantics.thy
@@ -1,27 +1,26 @@
 theory Example_Semantics
-imports "../Call_Return_Unfolding" "../Primitive_Matchers/IPSpace_Syntax"
+imports "../Call_Return_Unfolding" "../Primitive_Matchers/Common_Primitive_Matcher"
 begin
 
 
 section{*Examples Big Step Semantics*}
-text{*we use a primitive matcher which always apllies.*}
+text{*we use a primitive matcher which always applies.*}
   fun applies_Yes :: "('a, 'p) matcher" where
   "applies_Yes m p = True" 
   lemma[simp]: "Semantics.matches applies_Yes MatchAny p" by simp
   lemma[simp]: "Semantics.matches applies_Yes (Match e) p" by simp
 
   definition "m=Match (Src (Ip4Addr (0,0,0,0)))"
-  definition "p=\<lparr>src_ip=0, dst_ip=0, prot=protPacket.ProtTCP\<rparr>"
   lemma[simp]: "Semantics.matches applies_Yes m p" by (simp add: m_def)
 
   lemma "[''FORWARD'' \<mapsto> [(Rule m Log), (Rule m Accept), (Rule m Drop)]],applies_Yes,p\<turnstile>
       \<langle>[Rule MatchAny (Call ''FORWARD'')], Undecided\<rangle> \<Rightarrow> (Decision FinalAllow)"
   apply(rule call_result)
-  apply(auto)
+    apply(auto)
   apply(rule seq_cons)
-  apply(auto intro:Semantics.log)
+   apply(auto intro:Semantics.log)
   apply(rule seq_cons)
-  apply(auto intro: Semantics.accept)
+   apply(auto intro: Semantics.accept)
   apply(rule Semantics.decision)
   done
   
@@ -29,24 +28,24 @@ text{*we use a primitive matcher which always apllies.*}
           ''foo'' \<mapsto> [(Rule m Log), (Rule m Return)]],applies_Yes,p\<turnstile>
       \<langle>[Rule MatchAny (Call ''FORWARD'')], Undecided\<rangle> \<Rightarrow> (Decision FinalAllow)"
   apply(rule call_result)
-  apply(auto)
+    apply(auto)
   apply(rule seq_cons)
-  apply(auto intro: Semantics.log)
+   apply(auto intro: Semantics.log)
   apply(rule seq_cons)
-  apply(rule Semantics.call_return[where rs\<^sub>1="[Rule m Log]" and rs\<^sub>2="[]"])
-  apply(simp)+
-  apply(auto intro: Semantics.log)
+   apply(rule Semantics.call_return[where rs\<^sub>1="[Rule m Log]" and rs\<^sub>2="[]"])
+      apply(simp)+
+   apply(auto intro: Semantics.log)
   apply(auto intro: Semantics.accept)
   done
   
   lemma "[''FORWARD'' \<mapsto> [Rule m (Call ''foo''), Rule m Drop], ''foo'' \<mapsto> []],applies_Yes,p\<turnstile>
             \<langle>[Rule MatchAny (Call ''FORWARD'')], Undecided\<rangle> \<Rightarrow> (Decision FinalDeny)"
   apply(rule call_result)
-  apply(auto)
+    apply(auto)
   apply(rule Semantics.seq_cons)
-  apply(rule Semantics.call_result)
-  apply(auto)
-  apply(rule Semantics.skip)
+   apply(rule Semantics.call_result)
+     apply(auto)
+   apply(rule Semantics.skip)
   apply(auto intro: deny)
   done
 
@@ -54,31 +53,33 @@ text{*we use a primitive matcher which always apllies.*}
                     [Rule MatchAny (Call ''FORWARD'')]
          = [Rule (MatchAnd MatchAny m) Drop]" by eval
 
-  hide_const m p
+  hide_const m
+  
+  definition "pkt=\<lparr>p_iiface=''+'', p_oiface=''+'', p_src=0, p_dst=0, p_proto=TCP, p_sport=0, p_dport=0\<rparr>"
 
   text{*We tune the primitive matcher to support everything we need in the example. Note that the undefined cases cannot be handled with these exact semantics!*}
-  fun applies_exampleMatchExact :: "(iptrule_match, packet) matcher" where
-  "applies_exampleMatchExact (Src (Ip4Addr addr)) p \<longleftrightarrow> src_ip p = (ipv4addr_of_dotdecimal addr)" |
-  "applies_exampleMatchExact (Dst (Ip4Addr addr)) p \<longleftrightarrow> dst_ip p = (ipv4addr_of_dotdecimal addr)" |
-  "applies_exampleMatchExact (Prot ProtAll) p \<longleftrightarrow> True" |
-  "applies_exampleMatchExact (Prot ipt_protocol.ProtTCP) p \<longleftrightarrow> prot p = protPacket.ProtTCP" |
-  "applies_exampleMatchExact (Prot ipt_protocol.ProtUDP) p \<longleftrightarrow> prot p = protPacket.ProtUDP"
+  fun applies_exampleMatchExact :: "(common_primitive, simple_packet) matcher" where
+  "applies_exampleMatchExact (Src (Ip4Addr addr)) p \<longleftrightarrow> p_src p = (ipv4addr_of_dotdecimal addr)" |
+  "applies_exampleMatchExact (Dst (Ip4Addr addr)) p \<longleftrightarrow> p_dst p = (ipv4addr_of_dotdecimal addr)" |
+  "applies_exampleMatchExact (Prot ProtoAny) p \<longleftrightarrow> True" |
+  "applies_exampleMatchExact (Prot (Proto TCP)) p \<longleftrightarrow> p_proto p = TCP" |
+  "applies_exampleMatchExact (Prot (Proto UDP)) p \<longleftrightarrow> p_proto p = UDP"
   (*TODO, not exhaustive, only an example!!*)
 
   lemma "[''FORWARD'' \<mapsto> [ Rule (MatchAnd (Match (Src (Ip4Addr (0,0,0,0)))) (Match (Dst (Ip4Addr (0,0,0,0))))) Reject, 
                           Rule (Match (Dst (Ip4Addr (0,0,0,0)))) Log, 
-                          Rule (Match (Prot ipt_protocol.ProtTCP)) Accept,
-                          Rule (Match (Prot ipt_protocol.ProtTCP)) Drop]
-         ],applies_exampleMatchExact,\<lparr>src_ip=(ipv4addr_of_dotdecimal (1,2,3,4)), dst_ip=(ipv4addr_of_dotdecimal (0,0,0,0)), prot=protPacket.ProtTCP\<rparr>\<turnstile>
+                          Rule (Match (Prot (Proto TCP))) Accept,
+                          Rule (Match (Prot (Proto TCP))) Drop]
+         ],applies_exampleMatchExact, pkt\<lparr>p_src:=(ipv4addr_of_dotdecimal (1,2,3,4)), p_dst:=(ipv4addr_of_dotdecimal (0,0,0,0))\<rparr>\<turnstile>
             \<langle>[Rule MatchAny (Call ''FORWARD'')], Undecided\<rangle> \<Rightarrow> (Decision FinalAllow)"
   apply(rule call_result)
-  apply(auto)
+    apply(auto)
   apply(rule Semantics.seq_cons)
-  apply(auto intro: Semantics.nomatch simp add: ipv4addr_of_dotdecimal.simps ipv4addr_of_nat_def)
+   apply(auto intro: Semantics.nomatch simp add: ipv4addr_of_dotdecimal.simps ipv4addr_of_nat_def)
   apply(rule Semantics.seq_cons)
-  apply(auto intro: Semantics.log simp add: ipv4addr_of_dotdecimal.simps ipv4addr_of_nat_def)
+   apply(auto intro: Semantics.log simp add: ipv4addr_of_dotdecimal.simps ipv4addr_of_nat_def)
   apply(rule Semantics.seq_cons)
-  apply(auto intro: Semantics.accept)
+   apply(auto simp add: pkt_def intro: Semantics.accept)
   apply(auto intro: Semantics.decision)
   done
 
